# Problem
Verify these two identities regarding the gamma function that were given in the text
1. $\Gamma(\alpha + 1) = \alpha\Gamma(\alpha)$,
2. $\Gamma(1/2) = \sqrt{\pi}$.

# Solution
## (a)
Recall that for $\alpha > 0$ the Gamma function is defined as
$$
\Gamma(\alpha) = \int_0^\infty t^{\alpha - 1} e^{-t} dt
$$
applying integration by parts to $f'(t) = t^{\alpha - 1}, g(t) = e^{-t}$ where $f(t) = \frac{1}{\alpha}t^\alpha$ and $g'(t) = -e^{-t}$ yields
$$
\begin{aligned}
\int_0^\infty t^{\alpha - 1} e^{-t} dt &= \left[\frac{1}{\alpha}t^{\alpha}e^{-t}\right]_{t = 0}^{t = \infty} - \int_0^\infty \frac{1}{\alpha}t^\alpha (-e^{-t}) dt \\
&= \frac{1}{\alpha}\int_0^\infty t^\alpha e^{-t} dt \\
&= \frac{1}{\alpha} \int_0^\infty t^{(\alpha + 1) - 1} e^{-t} dt \\
&= \frac{1}{\alpha} \Gamma(\alpha),
\end{aligned}
$$
where we have used $t^\alpha = 0$ for $t = 0$ boundary and $e^{-t} = 0$ for $t = \infty$ boundary.

## (b)
To compute $\Gamma(1/2)$ we use the substitution $t = s^2, dt = 2s ds$ which preserves the integration boundries, with this substituion the integral becomes
$$
\Gamma(1/2) = \int_0^\infty (s^2)^{-1 / 2} e^{-s^2} 2s ds = 2\int_0^\infty e^{-s^2} ds.
$$
This is a classic integral which I will only sketch here, one way to compute is to note that $e^{-(x^2 + y^2)}$ is a radially symmetrical function and use the trick
$$
\begin{aligned}
\int_{-\infty}^\infty \int_{-\infty}^\infty e^{-(x^2 + y^2)} dx dx &= \left( \int_{-\infty}^\infty e^{-x^2} dx \right)^{2} \\
&= \left( 2 \int_0^\infty e^{-x^2} dx \right)^2
\end{aligned}
$$