# Problem
Verify the following identities.

(a) $$ A \setminus B = A \setminus (A \cap B) = A \cap B^c $$

(b) $$ B = (B \cap A) \cup (B \cap A^c) $$

(c) $$ B \setminus A = B \cap A^c $$

(d) $$ A \cup B = A \cup (B \cap A^c) $$


# Solution
## (a)
$$
\begin{aligned}
A \setminus B &= \{x : x \in A \setminus B\} \\
&= \{x : x \in A \wedge x \notin B\} \\
&= \{x : x \in A\} \cap {x : x \notin B} \\
&= A \cap B^C \\
&= A \cap (\Omega \setminus B) \\
&= A \cap (A \setminus B)
\end{aligned}
$$
## (b)
$$
\begin{aligned}
(B \cap A) \cup (B \cap A^c) &= \{x : x \in B \wedge x \in A\} \cup \{x : x \in B \wedge x \notin A\} \\
&= \{x : x \in B \wedge x \in A\} \cup \{x : x \in B \wedge x \notin A\} \\
&= \{x : (x \in B \wedge x \in A) \vee (x \in B \wedge x \notin A)\} \\
&= \{x : (x \in B) \wedge (x \in A \vee x \notin A)\} \\
&= \{x : x \ in B\} = B.
\end{aligned}
$$
## (c)
Already done in (a).
## (d)
$$
\begin{aligned}
A \cup B &= {x : x \in A \vee x \in B} \\
&= {x : x \in A \vee (x \in B \wedge x \notin A)} \\
&= A \cup (B \ A) \\
&= A \cup (B \cap A^c).
\end{aligned}
$$