# Problem
Verify the following identities for $n \geq 2$:

(a) 
$$
\sum_{k=0}^{n} (-1)^k \binom{n}{k} = 0
$$

(b)
$$
\sum_{k=1}^{n} k \binom{n}{k} = n2^{n-1}
$$

(c)
$$
\sum_{k=1}^{n} (-1)^{k+1} k \binom{n}{k} = 0
$$

# Solution
## (a)
For even $n$ this follows directly from the fact that
$$
\binom{n}{k} = \binom{n}{n - k}
$$

For the odd case, suppose $n + 1$ is odd. We claim, without proof, that the following identity holds:
$$
\binom{n + 1}{k + 1} = \binom{n}{k} + \binom{n + 1}{k}.
$$

With that we can write
$$
\begin{aligned}
1 + \sum_{k = 0}^n (-1)^{k + 1} \binom{n + 1}{k + 1} &= 1 + \sum­_{k = 0}^{n} (-1)^{k + 1} \left( \binom{n}{k} + \binom{n}{k + 1} \right) \\
&= 1 - \underbrace{\sum_{k = 0}^n \binom{n}{k}}_{= 0} + \sum_{k = 0}^n (-1)^{k + 1} \binom{n}{k + 1} \\
&= 1 + \sum_{k = 0}^n (-1)^{k + 1} \binom{n}{k + 1} \\
&= 1 + \sum_{k = 1}^n (-1)^k \binom{n}{k} \\
&= 1 - 1 + \underbrace{\sum_{k = 0}^n (-1)^k \binom{n}{k}}_{= 0} \\
&= 0
\end{aligned}
$$
where we have used that $n$ has to be even (as $n + 1$ is odd).

## (b)
We can write
$$
\begin{aligned}
\sum_{k = 1}^{n} k \binom{n}{k} &= \sum_{k = 1}^{n / 2} k \binom{n}{k} + (n - k) \underbrace{\binom{n}{n - k}}_{= \binom{n}{k}} \\
&= \sum­_{k = 1}^{n / 2} n \binom{n}{k} \\
&= n \sum_{k = 1}^{n / 2} \binom{n}{k} \\
&= n \frac{1}{2}\sum_{k = 1}^n \binom{n}{k} \\
&= n \frac{1}{2} 2^n = n2^{n - 1}.
\end{aligned}
$$