# Problem
Finish the proof of Theorem 1.1.4. For any events $A$, $B$, and $C$ defined on a sample space $S$, show that:

(a) $A \cup B = B \cup A$ and $A \cap B = B \cap A$ (commutativity)

(b) $A \cup (B \cup C) = (A \cup B) \cup C$ and $A \cap (B \cap C) = (A \cap B) \cap C$ (associativity)

(c) $(A \cup B)^c = A^c \cap B^c$ and $(A \cap B)^c = A^c \cup B^c$ (DeMorgan's Laws)

# Solution
## (a)
$$
\begin{aligned}
A \cup B &= \{x : x \in A \cup B\} \\
&= \{x : x \in A \vee x \in B\} \\
&= \{x : x \in B \vee x \in A\} \\
&= \{x : x \in B \cup A\} \\
&= B \cup A \\
A \cap B &= \{x : x \in A \cap B\} \\
&= \{x : x \in A \wedge x \in B\} \\
&= \{x : x \in B \wedge x \in A\} \\
&= \{x : x \in B \cap A\} \\
&= B \cap A.
\end{aligned}
$$
## (b)
$$
\begin{aligned}
A \cup (B \cup C) &= \{x : x \in A \vee x \in B \cup C\} \\
&= \{x : x \in A \vee (x \in B \vee x \in C)\} \\
&= \{x : \left(x \in A \vee x \in B \right) \vee \left( x \in A \vee x\in C \right) \} \\
&= \{x : x \in A \vee x \in B \} \cup \{x : x \in A \vee x \in C\} \\
&= (A \cup B) \cup (A \cup C).
\end{aligned}
$$
Using (a) we see that $A \cup (B \cup C) = (A \cup B) \cup (A \cup C) = (B \cup C) \cup A$ and the statement follows.

The proof for the intersection case is analogous.

## (c)
$$
\begin{aligned}
(A \cup B)^c &= \{x : x \notin A \cup B\} \\
&= \{x : \neg(x \in A \cup B)\} \\
&= \{x : \neg(x \in A \vee x \in B)\} \\
&= \{x : \neg(x \in A) \wedge \neg(x \in B)\} \\
&= \{x : x \notin A \wedge x \notin B\} = A^c \cap B^c.
\end{aligned}
$$

The other case is analogous.