In each of the following, find the pdf of $Y$. Show that the pdf integrates to 1.

(a) $Y = X^3$ and $f_X(x) = 42x^5(1-x), \ 0 < x < 1$

(b) $Y = 4X + 3$ and $f_X(x) = 7e^{-7x}, \ 0 < x < \infty$

(c) $Y = X^2$ and $f_X(x) = 30x^2(1 - x)^2, \ 0 < x < 1$

(See Example A.0.2 in Appendix A.)

# Solution
I will omit the integration to check if they integrate to 1.

## (a)
Note that $g(x) = x^3$ is a monotone increasing function, and therefore we can compute the pdf $f_Y$ of $Y$ by applying Theorem 2.1.5, noting that $g((0, 1)) = (0, 1)$
$$
f_Y(y) = f_X(g^{-1}(y)) \left| \frac{d}{dy} g^{-1}(y) \right|
$$
where, of course, $\frac{d}{dy} g^{-1}(y) = \frac{1}{3}g^{-2/3}$. In total this means that for $x = y^{1 / 3} = g(y)$ we have
$$
f_Y(y) = f_X(y^{1 / 3}) \frac{1}{3}y^{-2/3} = 42 (y^{1/3})^5(1 - y) = 14 y(1 - y^{1/3}).
$$

## (b)
Here we have $g(x) = 4x + 3$ or equivalently $\frac{1}{4}(g(x) - 3) = x$, i.e., $g^{-1}(y) = \frac{1}{4}(y - 3)$, whose derivative to constant $1 / 4$.

As such for $x = \frac{1}{4}(y - 3)$
$$
f_Y(y) = f_X\left(\frac{1}{4}(y - 3)\right) \frac{1}{4} = 7e^{-7(\frac{1}{4}(y - 3))} \frac{1}{4}
$$

Let $c := - 7 / 4$ then we have
$$
f_Y(y) = -ce^{cy - 3c}.
$$

## (c)
Here we have $x \in (0, 1)$ on which $g(x) = x^2$ is invertible with $g^{-1}(y) = + \sqrt{y} = y^{1 / 2}$. The derivative of this is inverse is $\frac{1}{2}y^{-1/2}$. With that we can compute
$$
\begin{aligned}
f_Y(y) &= f_X(y^{1 / 2}) \frac{1}{2}y^{-1/2} \\
&= 30y(1 - y^{1 / 2})^2 \frac{1}{2} y^{-1/2} \\
&= 15 y^{1/2}(1 - y^{1 / 2})^2.
\end{aligned}
$$